Cleanup, removed merge with arity 1

coq-osiris/examples/src/merge.ml
@@ -1,20 +1,11 @@
-let rec merge (l1, l2) =
+let rec merge l1 l2 =
   match l1, l2 with
   | [], l | l, [] -> l
   | h1::t1, h2::t2 ->
      if h1 <= h2 then
-       h1 :: (merge (t1, l2))
+       h1 :: (merge t1 l2)
      else
-       h2 :: (merge (l1, t2))
-
-let rec merge2 l1 l2 =
-  match l1, l2 with
-  | [], l | l, [] -> l
-  | h1::t1, h2::t2 ->
-     if h1 <= h2 then
-       h1 :: (merge2 t1 l2)
-     else
-       h2 :: (merge2 l1 t2)
+       h2 :: (merge l1 t2)
 
 let rec split l =
   match l with
@@ -32,5 +23,5 @@ let rec merge_sort l =
      let l1, l2 = split l in
      let l1' = merge_sort l1 in
      let l2' = merge_sort l2 in
-     merge2 l1' l2'
+     merge l1' l2'
 
